# 1 - Newton's Laws of Motion

```admonish textbook
John R. Taylor's _Classical Mechanics_ (2005)

---

Material used on this page:
- Chapter 1 - Newton's Laws of Motion
```

## Problems & Solutions

<h3 hidden><a class="header">Problem 1.1</a></h2>

```admonish problem title="Problem 1.1"
Given the two vectors $\vec{b} = \hat{x} + \hat{y}$ and $\vec{c} = \hat{x} + \hat{z}$ find

(a). $\vec{b} + \vec{c}$

(b). $5\vec{b} + 2\vec{c}$

(c). $\vec{b}\cdot\vec{c}$

(d). $\vec{b}\times\vec{c}$.
```
```admonish solution
(a). $\vec{b} + \vec{c} = \boxed{2\hat{x} + \hat{y} + \hat{z}}$

(b). $5\vec{b} + 2\vec{c} = \boxed{7\hat{x} + 5\hat{y} + 2\hat{z}}$

(c). $\vec{b}\cdot\vec{c} = (\hat{x} + \hat{y})\cdot(\hat{x} + \hat{z}) = \hat{x}\cdot\hat{x} = \boxed{1}$

(d).
$$
\begin{align}
\vec{b}\times\vec{c} &= (\hat{x} + \hat{y})\times(\hat{x} + \hat{z}) \\\\
                     &= \hat{x}\times\hat{z} + \hat{y}\times\hat{x} + \hat{y}\times\hat{z} \\\\
                     &= (-1)\hat{y} + (-1)\hat{z} + (1)\hat{x} \\\\
                     &= \boxed{\hat{x} - \hat{y} - \hat{z}}
\end{align}
$$
```

<h3 hidden><a class="header">Problem 1.2</a></h2>

```admonish problem title="Problem 1.2"
Two vectors are given as $\vec{b} = \hat{x} + 2\hat{y} + 3\hat{z}$ and $\vec{c} = 3\hat{x} + 2\hat{y} + \hat{z}$. Find

(a). $\vec{b} + \vec{c}$

(b). $5\vec{b} - 2\vec{c}$

(c). $\vec{b}\times\vec{c}$.
```
```admonish solution
(a). $\vec{b} + \vec{c} = \boxed{4\hat{x} + 4\hat{y} + 4\hat{z}}$

(b). $5\vec{b} - 2\vec{c} = 5(\hat{x} + 2\hat{y} + 3\hat{z}) - 2(3\hat{x} + 2\hat{y} + \hat{z}) = \boxed{-\hat{x} + 6\hat{y} + 13\hat{z}}$

(c).
$$
\begin{align}
\vec{b}\times\vec{c} &= (\hat{x} + 2\hat{y} + 3\hat{z})\times(3\hat{x} + 2\hat{y} + \hat{z}) \\\\
                     &= (1 * 2)\hat{x}\times\hat{y} + (1 * 1)\hat{x}\times\hat{z} + (2 * 3)\hat{y}\times\hat{x} \\\\
                     &\phantom{=} + (2 * 1)\hat{y}\times\hat{z} + (3 * 3)\hat{z}\times\hat{x} + (3 * 2)\hat{z}\times \hat{y} \\\\
                     &= (2)\hat{z} + (1)(-\hat{y}) + (6)(-\hat{z}) + (2)\hat{x} + (9)\hat{y} + (6)(-\hat{x}) \\\\
                     &= \boxed{-4\hat{x} + 8\hat{y} - 4\hat{z}}
\end{align}
$$
```
